{
  "nbformat": 4,
  "nbformat_minor": 0,
  "metadata": {
    "colab": {
      "provenance": [],
      "authorship_tag": "ABX9TyNur6Dcefkn7m6E78UZ7UwH"
    },
    "kernelspec": {
      "name": "python3",
      "display_name": "Python 3"
    },
    "language_info": {
      "name": "python"
    }
  },
  "cells": [
    {
      "cell_type": "markdown",
      "source": [
        "# 20. Limits of Real Functions\n",
        "\n",
        "1. Compute:\n",
        "$$\\lim_{x \\to \\infty} \\frac{x^3 + 2x^2}{x^4 - 3x^3}$$\n",
        "\n",
        "2. Find:\n",
        "$$\\lim_{x \\to 0} \\frac{\\sin(3x)}{2x + 1}$$\n",
        "\n",
        "3. Find the asymptotes of the function:\n",
        "$$f(x) = \\frac{x^2 - 1}{x^2 + 1}, \\quad g(x) = \\frac{\\sin(x)}{x^2 + 1}.$$\n",
        "\n",
        "-------\n",
        "\n",
        "\n",
        "### 1. Compute:\n",
        "$$\\lim_{x \\to \\infty} \\frac{x^3 + 2x^2}{x^4 - 3x^3}$$\n",
        "\n",
        "**Solution:**\n",
        "\n",
        "We can divide both the numerator and the denominator by \\( x^4 \\), the highest power of \\( x \\) in the denominator:\n",
        "\n",
        "$$\n",
        "\\lim_{x \\to \\infty} \\frac{x^3 + 2x^2}{x^4 - 3x^3} = \\lim_{x \\to \\infty} \\frac{\\frac{x^3}{x^4} + \\frac{2x^2}{x^4}}{\\frac{x^4}{x^4} - \\frac{3x^3}{x^4}}\n",
        "$$\n",
        "\n",
        "Simplifying the terms:\n",
        "\n",
        "$$\n",
        "= \\lim_{x \\to \\infty} \\frac{\\frac{1}{x} + \\frac{2}{x^2}}{1 - \\frac{3}{x}}\n",
        "$$\n",
        "\n",
        "As $$ x \\to \\infty , both  \\frac{1}{x}  and  \\frac{2}{x^2}  approach 0, and  \\frac{3}{x} $$ also approaches 0:\n",
        "\n",
        "$$\n",
        "= \\frac{0 + 0}{1 - 0} = 0\n",
        "$$\n",
        "\n",
        "So, the limit is:\n",
        "\n",
        "$$\n",
        "\\lim_{x \\to \\infty} \\frac{x^3 + 2x^2}{x^4 - 3x^3} = 0\n",
        "$$\n",
        "\n",
        "---\n",
        "\n",
        "### 2. Find:\n",
        "$$\\lim_{x \\to 0} \\frac{\\sin(3x)}{2x + 1}$$\n",
        "\n",
        "**Solution:**\n",
        "\n",
        "We use the fact that $$ \\lim_{x \\to 0} \\frac{\\sin(x)}{x} = 1 $$ and recognize that $$( 3x \\to 0 ) as ( x \\to 0 ):$$\n",
        "\n",
        "$$\n",
        "\\lim_{x \\to 0} \\frac{\\sin(3x)}{2x + 1}\n",
        "$$\n",
        "\n",
        "First, we observe that $$( \\sin(3x) \\to 0 \\\n",
        " $$as\n",
        "$$( x \\to 0 ), and ( 2x + 1 \\to 1 ) as ( x \\to 0 ).$$\n",
        "\n",
        "Thus:\n",
        "\n",
        "$$\n",
        "\\lim_{x \\to 0} \\frac{\\sin(3x)}{2x + 1} = \\frac{0}{1} = 0\n",
        "$$\n",
        "\n",
        "So, the limit is:\n",
        "\n",
        "$$\n",
        "\\lim_{x \\to 0} \\frac{\\sin(3x)}{2x + 1} = 0\n",
        "$$\n",
        "\n",
        "---\n",
        "\n",
        "### 3. Find the asymptotes of the functions:\n",
        "$$\n",
        " ( f(x) = \\frac{x^2 - 1}{x^2 + 1} )\n",
        "$$\n",
        "$$\n",
        " ( g(x) = \\frac{\\sin(x)}{x^2 + 1} )\n",
        "$$\n",
        "\n",
        "#### **For $$( f(x) = \\frac{x^2 - 1}{x^2 + 1} )$$:**\n",
        "\n",
        "**Vertical Asymptotes:**\n",
        "\n",
        "The function \\( f(x) \\) has vertical asymptotes where the denominator equals 0. However, the denominator $$( x^2 + 1 ) $$never equals 0 for any real value of \\( x \\), so there are **no vertical asymptotes**.\n",
        "\n",
        "**Horizontal Asymptotes:**\n",
        "\n",
        "As $$( x \\to \\infty )$$, the degree of the numerator and the denominator is the same (both are degree 2). Therefore, the horizontal asymptote is the ratio of the leading coefficients:\n",
        "\n",
        "$$\n",
        "\\lim_{x \\to \\infty} f(x) = \\lim_{x \\to \\infty} \\frac{x^2 - 1}{x^2 + 1} = \\frac{1}{1} = 1\n",
        "$$\n",
        "\n",
        "Thus, the horizontal asymptote is:\n",
        "\n",
        "$$\n",
        "y = 1\n",
        "$$\n",
        "\n",
        "#### **For $$( g(x) = \\frac{\\sin(x)}{x^2 + 1} )$$:**\n",
        "\n",
        "**Vertical Asymptotes:**\n",
        "\n",
        "The function \\( g(x) \\) has vertical asymptotes where the denominator equals 0. Since $$ ( x^2 + 1 = 0 )$$ has no real solutions, there are **no vertical asymptotes**.\n",
        "\n",
        "**Horizontal Asymptotes:**\n",
        "\n",
        "As \\( x \\to \\infty \\), we can observe that $$( sin(x) ) $$oscillates between -1 and 1, while $$( x^2 + 1 \\to \\infty )$$. Therefore, the function $$( g(x) )$$ approaches 0 as \\( x \\to \\infty \\):\n",
        "\n",
        "$$\n",
        "\\lim_{x \\to \\infty} g(x) = \\lim_{x \\to \\infty} \\frac{\\sin(x)}{x^2 + 1} = 0\n",
        "$$\n",
        "\n",
        "Thus, the horizontal asymptote is:\n",
        "\n",
        "$$\n",
        "y = 0\n",
        "$$\n",
        "\n",
        "### Final Answers:\n",
        "\n",
        "- For ( f(x) = $$\\frac{x^2 - 1}{x^2 + 1} $$ there is a **horizontal asymptote** at ( y = 1 ) and **no vertical asymptotes**.\n",
        "\n",
        "- For ( g(x) = $$\\frac{\\sin(x)}{x^2 + 1} $$ there is a **horizontal asymptote** at ( y = 0 ) and **no vertical asymptotes**.\n",
        "\n",
        "\n",
        "https://www.geogebra.org/calculator/phqjx99m\n",
        "\n",
        "\n"
      ],
      "metadata": {
        "id": "fOH2LhpZbENg"
      }
    }
  ]
}