{
  "nbformat": 4,
  "nbformat_minor": 0,
  "metadata": {
    "colab": {
      "provenance": [],
      "authorship_tag": "ABX9TyMblKN2foHZnSq4sNcOIJkS"
    },
    "kernelspec": {
      "name": "python3",
      "display_name": "Python 3"
    },
    "language_info": {
      "name": "python"
    }
  },
  "cells": [
    {
      "cell_type": "markdown",
      "source": [
        "FUNCTIONS\n",
        "\n",
        "---\n",
        "\n",
        "1. Draw in a single GeoGebra notebook the following functions:\n",
        "\n",
        "   $$\n",
        "   f(x) = x^2\n",
        "   $$\n",
        "\n",
        "   $$\n",
        "   g(x) = \\sqrt{x}\n",
        "   $$\n",
        "\n",
        "   $$\n",
        "   h(x) = \\frac{1}{x}\n",
        "   $$\n",
        "\n",
        "   $$\n",
        "   j(x) = \\sin(x)\n",
        "   $$\n",
        "\n",
        "   Find the value of all the above functions at $x = 2$.\n",
        "\n",
        "2. Let $f(x) = 3x - 1$ and $g(x) = \\sqrt{x}$. Find:\n",
        "\n",
        "   - $f(g(x))$\n",
        "   - $g(f(x))$\n",
        "   - $f(f(x))$\n",
        "   - $g(g(x))$\n",
        "\n",
        "   Visualize the functions in a single GeoGebra notebook.\n",
        "\n",
        "3. Let $f(x) = e^x$ and $g(x) = \\ln(x)$. Check $f(g(x))$ and $g(f(x))$. What do you notice?\n",
        "\n",
        "4. We have the function $f = \\{(1, 7), (2, 9), (3, 11)\\}$. Give the inverse function $f^{-1}$.\n",
        "\n",
        "5. We have the function $f = \\{(1, 7), (2, 7), (3, 11)\\}$. Give the inverse function $f^{-1}$.\n",
        "\n",
        "6. We have the function $f(x) = x - 1$. Give the inverse function $f^{-1}$. Show both functions on the same GeoGebra notebook.\n",
        "\n",
        "\n"
      ],
      "metadata": {
        "id": "rdUHT22iQKFq"
      }
    },
    {
      "cell_type": "markdown",
      "source": [
        "# **1**.\n",
        "\n",
        "\n",
        "https://www.geogebra.org/calculator/wyubkgrb\n",
        "\n",
        "# **2**.\n",
        "Hereâ€™s the solution correctly formatted for Google Colab using \\$...\\$ for inline math and \\$\\$...\\$\\$ for display math:\n",
        "\n",
        "---\n",
        "\n",
        "### 1. **Find \\( f(g(x)) \\):**\n",
        "\n",
        "We are given \\( f(x) = 3x - 1 \\) and \\( g(x) =$$ \\sqrt{x} $$\n",
        "\n",
        "$$\n",
        "f(g(x)) = f(\\sqrt{x}) = 3\\sqrt{x} - 1\n",
        "$$\n",
        "\n",
        "So:\n",
        "$$\n",
        "f(g(x)) = 3\\sqrt{x} - 1\n",
        "$$\n",
        "\n",
        "---\n",
        "\n",
        "### 2. **Find \\( g(f(x)) \\):**\n",
        "\n",
        "We are given \\( f(x) = 3x - 1 \\) and \\( g(x) = $$\\sqrt{x} .$$\n",
        "\n",
        "$$\n",
        "g(f(x)) = g(3x - 1) = \\sqrt{3x - 1}\n",
        "$$\n",
        "\n",
        "Thus:\n",
        "$$\n",
        "g(f(x)) = \\sqrt{3x - 1}\n",
        "$$\n",
        "\n",
        "---\n",
        "\n",
        "### 3. **Find \\( f(f(x)) \\):**\n",
        "\n",
        "We are given \\( f(x) = 3x - 1 \\).\n",
        "\n",
        "$$\n",
        "f(f(x)) = f(3x - 1) = 3(3x - 1) - 1\n",
        "$$\n",
        "\n",
        "Simplify:\n",
        "$$\n",
        "f(f(x)) = 9x - 3 - 1 = 9x - 4\n",
        "$$\n",
        "\n",
        "So:\n",
        "$$\n",
        "f(f(x)) = 9x - 4\n",
        "$$\n",
        "\n",
        "---\n",
        "\n",
        "### 4. **Find \\( g(g(x)) \\):**\n",
        "\n",
        "We are given \\ g(x) = $$\\sqrt{x} $$.\n",
        "\n",
        "$$\n",
        "g(g(x)) = g(\\sqrt{x}) = \\sqrt{\\sqrt{x}} = x^{1/4}\n",
        "$$\n",
        "\n",
        "Thus:\n",
        "$$\n",
        "g(g(x)) = x^{1/4}\n",
        "$$\n",
        "\n",
        "---\n",
        "\n",
        "### Final Results:\n",
        "\n",
        "$$\n",
        "\\begin{aligned}\n",
        "f(g(x)) &= 3\\sqrt{x} - 1, \\\\\n",
        "g(f(x)) &= \\sqrt{3x - 1}, \\\\\n",
        "f(f(x)) &= 9x - 4, \\\\\n",
        "g(g(x)) &= x^{1/4}.\n",
        "\\end{aligned}\n",
        "$$\n",
        "\n",
        "\n",
        "https://www.geogebra.org/calculator/gmhmpudh\n",
        "\n",
        "\n",
        "# **3.**\n",
        "\n",
        "\n",
        "\n",
        "### 1. **Find \\( f(g(x)) \\):**\n",
        "\n",
        "We are given \\( f(x) = e^x \\) and \\( g(x) = \\ln(x) \\).\n",
        "\n",
        "$$\n",
        "f(g(x)) = f(\\ln(x)) = e^{\\ln(x)}\n",
        "$$\n",
        "\n",
        "We know that \\( e^{\\ln(x)} = x \\), so:\n",
        "\n",
        "$$\n",
        "f(g(x)) = x\n",
        "$$\n",
        "\n",
        "---\n",
        "\n",
        "### 2. **Find \\( g(f(x)) \\):**\n",
        "\n",
        "We are given \\( f(x) = e^x \\) and \\( g(x) = \\ln(x) \\).\n",
        "\n",
        "$$\n",
        "g(f(x)) = g(e^x) = \\ln(e^x)\n",
        "$$\n",
        "\n",
        "We know that \\( \\ln(e^x) = x \\), so:\n",
        "\n",
        "$$\n",
        "g(f(x)) = x\n",
        "$$\n",
        "\n",
        "---\n",
        "\n",
        "### Observation:\n",
        "\n",
        "- \\( f(g(x)) = x \\)\n",
        "- \\( g(f(x)) = x \\)\n",
        "\n",
        "Thus, for these functions, the compositions \\( f(g(x)) \\) and \\( g(f(x)) \\) yield the identity function \\( x \\), meaning they \"undo\" each other. This is a special property of the exponential and logarithmic functions: they are inverses of each other.\n",
        "\n",
        "\n",
        "# **4.**\n",
        "\n",
        "To find the inverse function \\( f^{-1} \\), we simply swap the coordinates in each pair from the original function \\( f \\). The function \\( f = \\{(1, 7), (2, 9), (3, 11)\\} \\) consists of the following pairs:\n",
        "\n",
        "- \\( (1, 7) \\)\n",
        "- \\( (2, 9) \\)\n",
        "- \\( (3, 11) \\)\n",
        "\n",
        "Now, to find \\( f^{-1} \\), we swap each pair:\n",
        "\n",
        "- \\( (7, 1) \\)\n",
        "- \\( (9, 2) \\)\n",
        "- \\( (11, 3) \\)\n",
        "\n",
        "Thus, the inverse function is:\n",
        "\n",
        "$$\n",
        "f^{-1} = \\{(7, 1), (9, 2), (11, 3)\\}\n",
        "$$\n",
        "\n",
        "This means that in \\( f^{-1} \\), the input is the output of \\( f \\), and the output is the input of \\( f \\).\n",
        "\n",
        "\n",
        "# **5.**\n",
        "\n",
        "For a function to have an inverse, it must be **one-to-one** (meaning each input corresponds to exactly one output).\n",
        "\n",
        " The function \\( f = \\{(1, 7), (2, 7), (3, 11)\\} \\) is\n",
        " not one-to-one\n",
        " because both \\( 1 \\) and \\( 2 \\) map to the same value, \\( 7 \\).\n",
        "\n",
        "Since a function is not one-to-one if two distinct inputs map to the same output, this function does **not** have an inverse.\n",
        "\n",
        "In other words, the inverse function $$ f^{-1} $$ does not exist in this case.\n",
        "\n",
        "\n",
        "\n",
        "\n",
        "# **6.**\n",
        "---\n",
        "\n",
        "### Finding the Inverse of \\( f(x) = x - 1 \\):\n",
        "\n",
        "To find the inverse of \\( f(x) = x - 1 \\), follow these steps:\n",
        "\n",
        "1. Replace \\( f(x) \\) with \\( y \\):\n",
        "   $$ y = x - 1 $$\n",
        "\n",
        "2. Swap \\( x \\) and \\( y \\) to get the inverse:\n",
        "   $$ x = y - 1 $$\n",
        "\n",
        "3. Solve for \\( y \\):\n",
        "   $$ y = x + 1 $$\n",
        "\n",
        "So, the inverse function is:\n",
        "$$ f^{-1}(x) = x + 1 $$\n",
        "\n",
        "---\n",
        "\n",
        "https://www.geogebra.org/calculator/xqdxtveh\n"
      ],
      "metadata": {
        "id": "G6lA6jHXSTco"
      }
    },
    {
      "cell_type": "code",
      "source": [],
      "metadata": {
        "id": "VqEWLqosdJdQ"
      },
      "execution_count": null,
      "outputs": []
    }
  ]
}