{
  "nbformat": 4,
  "nbformat_minor": 0,
  "metadata": {
    "colab": {
      "provenance": []
    },
    "kernelspec": {
      "name": "python3",
      "display_name": "Python 3"
    },
    "language_info": {
      "name": "python"
    }
  },
  "cells": [
    {
      "cell_type": "markdown",
      "source": [
        "\n",
        "# 25. Differential Equations\n",
        "\n",
        "## 1. Solve the following first-order ordinary differential equations:\n",
        "\n",
        "- $$ y'(x) = y(x) $$\n",
        "- $$ y'(x) = \\frac{1}{2y(x)} $$\n",
        "\n",
        "## 2. Solve the first-order ordinary differential equations using the method of separation of variables for \\( x \\) and \\( y = y(x) \\):\n",
        "\n",
        "- $$ \\frac{dy}{dx} = \\frac{x}{y} $$\n",
        "- $$ \\frac{dy}{dx} = \\frac{y}{x} $$\n",
        "- $$ \\frac{dy}{dx} = xy $$\n",
        "\n",
        "## 3. Solve the second-order ordinary differential equations:\n",
        "\n",
        "- $$ y''(x) + y'(x) = 0, \\quad \\text{with boundary conditions } y(0) = 2 \\text{ and } y'(0) = -1 $$\n",
        "- $$ y''(x) - y(x) = 0, \\quad \\text{with boundary conditions } y(0) = 2 \\text{ and } y'(0) = 0 $$\n",
        "- $$ \\frac{d^2y(x)}{dx^2} = -\\omega^2 y(x) $$\n",
        "\n",
        "## 4. Check if the function\n",
        "\n",
        "$$ \\psi(t, x) = A \\cos(\\omega t + kx) $$\n",
        "\n",
        "is a solution of the second-order partial differential equation (the so-called \"wave equation\"), where\n",
        "\n",
        "$$ v = \\frac{\\omega}{k} = \\frac{2\\pi / T}{2\\pi / \\lambda} $$\n",
        "\n",
        "and\n",
        "\n",
        "$$ \\frac{\\partial^2 \\psi(t, x)}{\\partial t^2} - v^2 \\frac{\\partial^2 \\psi(t, x)}{\\partial x^2} = 0. $$\n",
        "\n",
        "\n",
        "\n",
        "\n",
        "---\n",
        "\n",
        "## **1. Solve the first-order ODEs:**\n",
        "\n",
        "### **(i) \\( y'(x) = y(x) \\)**\n",
        "\n",
        "$$ \\frac{dy}{dx} = y $$\n",
        "\n",
        "Separation of variables:\n",
        "\n",
        "$$ \\frac{dy}{y} = dx $$\n",
        "\n",
        "Integrating both sides:\n",
        "\n",
        "$$ \\ln |y| = x + C $$\n",
        "\n",
        "Solving for \\( y \\):\n",
        "\n",
        "$$ y = C e^x $$\n",
        "\n",
        "---\n",
        "\n",
        "### **(ii) $( y'(x) = \\frac{1}{2y(x)} )$**\n",
        "\n",
        "$$ \\frac{dy}{dx} = \\frac{1}{2y} $$\n",
        "\n",
        "Separation of variables:\n",
        "\n",
        "$$ 2y \\, dy = dx $$\n",
        "\n",
        "Integrating both sides:\n",
        "\n",
        "$$ \\int 2y \\, dy = \\int dx $$\n",
        "\n",
        "$$ y^2 = x + C $$\n",
        "\n",
        "$$ y = \\pm\\sqrt{x + C} $$\n",
        "\n",
        "---\n",
        "\n",
        "## **2. Solve by separation of variables:**\n",
        "\n",
        "### **(i) $( \\frac{dy}{dx} = \\frac{x}{y} )$**\n",
        "\n",
        "$$ y \\, dy = x \\, dx $$\n",
        "\n",
        "Integrating:\n",
        "\n",
        "$$ \\int y \\, dy = \\int x \\, dx $$\n",
        "\n",
        "$$ \\frac{y^2}{2} = \\frac{x^2}{2} + C $$\n",
        "\n",
        "$$ y^2 = x^2 + 2C $$\n",
        "\n",
        "$$ y = \\pm\\sqrt{x^2 + 2C} $$\n",
        "\n",
        "---\n",
        "\n",
        "### **(ii) $( \\frac{dy}{dx} = \\frac{y}{x} )$**\n",
        "\n",
        "$$ \\frac{dy}{y} = \\frac{dx}{x} $$\n",
        "\n",
        "Integrating:\n",
        "\n",
        "$$ \\ln |y| = \\ln |x| + C $$\n",
        "\n",
        "$$ y = Cx $$\n",
        "\n",
        "---\n",
        "\n",
        "### **(iii) $( \\frac{dy}{dx} = xy )\\$**\n",
        "\n",
        "$$ \\frac{dy}{y} = x \\, dx $$\n",
        "\n",
        "Integrating:\n",
        "\n",
        "$$ \\ln |y| = \\frac{x^2}{2} + C $$\n",
        "\n",
        "$$ y = e^C e^{x^2/2} = C e^{x^2/2} $$\n",
        "\n",
        "---\n",
        "\n",
        "## **3. Solve second-order ODEs:**\n",
        "\n",
        "### **(i) \\( y''(x) + y'(x) = 0 \\), with \\( y(0) = 2 \\), \\( y'(0) = -1 \\)**\n",
        "\n",
        "Characteristic equation:\n",
        "\n",
        "$$ r^2 + r = 0 $$\n",
        "\n",
        "$$ r(r + 1) = 0 $$\n",
        "\n",
        "$$ r = 0, -1 $$\n",
        "\n",
        "General solution:\n",
        "\n",
        "$$ y(x) = C_1 + C_2 e^{-x} $$\n",
        "\n",
        "Using \\( y(0) = 2 \\):\n",
        "\n",
        "$$ C_1 + C_2 = 2 $$\n",
        "\n",
        "Derivative:\n",
        "\n",
        "$$ y'(x) = -C_2 e^{-x} $$\n",
        "\n",
        "Using \\( y'(0) = -1 \\):\n",
        "\n",
        "$$ - C_2 = -1 \\Rightarrow C_2 = 1 $$\n",
        "\n",
        "Thus, \\( C_1 = 1 \\), and the final solution is:\n",
        "\n",
        "$$ y(x) = 1 + e^{-x} $$\n",
        "\n",
        "---\n",
        "\n",
        "### **(ii) \\( y''(x) - y(x) = 0 \\), with \\( y(0) = 2 \\), \\( y'(0) = 0 \\)**\n",
        "\n",
        "Characteristic equation:\n",
        "\n",
        "$$ r^2 - 1 = 0 $$\n",
        "\n",
        "$$ r = \\pm1 $$\n",
        "\n",
        "General solution:\n",
        "\n",
        "$$ y(x) = C_1 e^x + C_2 e^{-x} $$\n",
        "\n",
        "Using \\( y(0) = 2 \\):\n",
        "\n",
        "$$ C_1 + C_2 = 2 $$\n",
        "\n",
        "Derivative:\n",
        "\n",
        "$$ y'(x) = C_1 e^x - C_2 e^{-x} $$\n",
        "\n",
        "Using \\( y'(0) = 0 \\):\n",
        "\n",
        "$$ C_1 - C_2 = 0 $$\n",
        "\n",
        "$$ C_1 = C_2 $$\n",
        "\n",
        "Solving:\n",
        "\n",
        "$$ C_1 + C_1 = 2 \\Rightarrow 2C_1 = 2 \\Rightarrow C_1 = 1, C_2 = 1 $$\n",
        "\n",
        "Final solution:\n",
        "\n",
        "$$ y(x) = e^x + e^{-x} $$\n",
        "\n",
        "---\n",
        "\n",
        "### **(iii) $( y''(x) = -\\omega^2 y(x) \\$**\n",
        "\n",
        "Characteristic equation:\n",
        "\n",
        "$$ r^2 + \\omega^2 = 0 $$\n",
        "\n",
        "$$ r = \\pm i\\omega $$\n",
        "\n",
        "General solution:\n",
        "\n",
        "$$ y(x) = C_1 \\cos(\\omega x) + C_2 \\sin(\\omega x) $$\n",
        "\n",
        "---\n",
        "\n",
        "## **4. Verify $( \\psi(t, x) = A \\cos(\\omega t + kx) \\$ satisfies the wave equation**\n",
        "\n",
        "Given PDE:\n",
        "\n",
        "$$ \\frac{\\partial^2 \\psi}{\\partial t^2} - v^2 \\frac{\\partial^2 \\psi}{\\partial x^2} = 0 $$\n",
        "\n",
        "Compute $( \\frac{\\partial^2 \\psi}{\\partial t^2} )$:\n",
        "\n",
        "$$ \\psi(t, x) = A \\cos(\\omega t + kx) $$\n",
        "\n",
        "First derivative:\n",
        "\n",
        "$$ \\frac{\\partial \\psi}{\\partial t} = -A \\omega \\sin(\\omega t + kx) $$\n",
        "\n",
        "Second derivative:\n",
        "\n",
        "$$ \\frac{\\partial^2 \\psi}{\\partial t^2} = -A \\omega^2 \\cos(\\omega t + kx) $$\n",
        "\n",
        "Compute $( \\frac{\\partial^2 \\psi}{\\partial x^2} )\\$:\n",
        "\n",
        "First derivative:\n",
        "\n",
        "$$ \\frac{\\partial \\psi}{\\partial x} = -A k \\sin(\\omega t + kx) $$\n",
        "\n",
        "Second derivative:\n",
        "\n",
        "$$ \\frac{\\partial^2 \\psi}{\\partial x^2} = -A k^2 \\cos(\\omega t + kx) $$\n",
        "\n",
        "Check the wave equation:\n",
        "\n",
        "$$ \\frac{\\partial^2 \\psi}{\\partial t^2} - v^2 \\frac{\\partial^2 \\psi}{\\partial x^2} = -A \\omega^2 \\cos(\\omega t + kx) + v^2 A k^2 \\cos(\\omega t + kx) $$\n",
        "\n",
        "Since $( v = \\frac{\\omega}{k} \\$, then $ v^2 = $\\frac{\\omega^2}{k^2}$ \\$, so:\n",
        "\n",
        "$$ -A \\omega^2 \\cos(\\omega t + kx) + A \\omega^2 \\cos(\\omega t + kx) = 0 $$\n",
        "\n",
        "Thus, $ \\psi(t, x)$ satisfies the wave equation. âœ…"
      ],
      "metadata": {
        "id": "Dwr8jbhk_-51"
      }
    },
    {
      "cell_type": "code",
      "execution_count": null,
      "metadata": {
        "id": "fSZCgXgD_bkc"
      },
      "outputs": [],
      "source": []
    }
  ]
}